src/Helpers_VmSemantics.v
@@ -109,6 +109,7 @@ Proof.
         jkjk'; eauto. 
   -
     repeat (df; dohtac; df; try tauto).
+    
 Defined.
 
 Ltac do_pl_immut :=
