src/MonadVM.v
@@ -63,12 +63,21 @@ Definition add_trace (tr':list Ev) : cvm_st -> cvm_st :=
 Definition add_tracem (tr:list Ev) : CVM unit :=
   modify (add_trace tr).
 
-
-Definition split_evm (i:nat) (sp1 sp2:SP) (e:EvidenceC) (p:Plc) : CVM (EvidenceC*EvidenceC) :=
+Definition split_ev_seq (i:nat) (sp1 sp2:SP) (e:EvidenceC) (p:Plc) : CVM (EvidenceC*EvidenceC) :=
     let e1 := splitEv sp1 e in
     let e2 := splitEv sp2 e in
     add_tracem [Term.split i p] ;;
                ret (e1,e2).
+
+Definition split_ev_par (i:nat) (sp1 sp2:SP) (t1 t2:AnnoTerm) (e:EvidenceC) (p:Plc) : CVM (Loc*Loc) :=
+    let e1 := splitEv sp1 e in
+    let e2 := splitEv sp2 e in
+    let loc_e1 := fst (range t1) in
+    let loc_e2 := fst (range t2) in
+    put_store_at loc_e1 e1 ;;
+    put_store_at loc_e2 e2 ;;
+    add_tracem [Term.splitp i loc_e1 loc_e2 p] ;;
+    ret (loc_e1,loc_e2).
 
 (** * Partially-symbolic implementations of IO operations *)
 
@@ -153,9 +162,11 @@ Definition join_seq (n:nat) (p:Plc) (e1:EvidenceC) (e2:EvidenceC) : CVM unit :=
   put_ev (ssc e1 e2) ;;
   add_tracem [Term.join n p].
 
-Definition join_par (n:nat) (p:Plc) (e1:EvidenceC) (e2:EvidenceC) : CVM unit :=
-  put_ev (ppc e1 e2) ;;
-  add_tracem [Term.join n p].
+Definition join_par (n:nat) (p:Plc) (xi:Loc) (yi:Loc) (*(e1:EvidenceC) (e2:EvidenceC)*) : CVM unit :=
+  e1r <- get_store_at xi ;;
+  e2r <- get_store_at yi ;;
+  put_ev (ppc e1r e2r) ;;
+  add_tracem [Term.joinp n xi yi p].
   
 
 (** * Helper functions for Appraisal *)
@@ -212,7 +223,8 @@ Ltac monad_unfold :=
   get_pl,
   add_tracem,
   modify_evm,
-  split_evm,
+  split_ev_seq,
+  join_par,
   add_trace,
   failm,
   (* Uncommenting these evaluates too much, can't apply lemmas *)
